curien.v
@@ -1,13 +1,13 @@
-Require Import Unicode.Utf8 List db util.  
+Require Import util db.  
 Import ListNotations. 
 
 Inductive closure := | close : tm → list closure → closure. 
 Definition env := list closure.
 
 Inductive step : closure → closure → Type := 
-  | abs : ∀ b e, step (close (lam b) e) (close (lam b) e)
-  | var : ∀ x e v c, nth_error e x = Some c → step c v → step (close (var x) e) v
-  | app : ∀ m n b e v mve, 
+  | Abs : ∀ b e, step (close (lam b) e) (close (lam b) e)
+  | Var : ∀ x e v c, nth_error e x = Some c → step c v → step (close (var x) e) v
+  | App : ∀ m n b e v mve, 
       step (close m e) (close (lam b) mve) → 
       step (close b (close n e::mve)) v → 
       step (close (app m n) e) v.
