cem_cesm.v
@@ -1,6 +1,4 @@
-Require Import cem cesm relations List.
-Require Import Unicode.Utf8.
-Require cem cesm.
+Require Import cem cesm relations util.
 
 Notation " c1 '→_s*' c2 " := (refl_trans_clos cesm.step c1 c2) (at level 30). 
 
@@ -10,27 +8,28 @@ Definition b2s (c : configuration) : stack → state := match c with
 Definition convert_to_cesm (c c' : configuration) : Type := match (c, c') with
   | (conf h c, conf h' c') => ∀ s, (st h s c) →_s* (st h' s c') end.
 
-Lemma cem_cesm : ∀ c v, c ⇓ v → ∀ s, b2s c s →_s* b2s v s. 
-intros c v H. induction H.
+Lemma cem_cesm : ∀ Φ Ψ c v, conf Φ c ⇓ conf Ψ v → ∀ s, st Φ s c →_s* st Ψ s v. 
+intros. induce X; intros; invert H1; invert H0. 
 (* Var *)
-- simpl. simpl in IHstep. intros. rename y into Y.  
-  apply t_step with (y:=[Υ ++ x ↦ {M, Y} :: Φ, inr x :: s]M). auto. 
-  + apply Var. assumption. 
-  + apply t_step2 with (y:= [Υ ++ x ↦ {M, Y} :: Ψ, inr x :: s](close (db.lam B) e)). 
-    * apply Upd. 
-    * auto. 
+- destruct v0. apply values_only in X. inversion X. 
+  specialize (IHX _ _ _ _ (inr x::s) eq_refl eq_refl).   
+  apply t_step with (y0:=[Φ0, inr x :: s]M). 
+  + apply Var with (e':=z). assumption. 
+  + apply t_step2 with (y0:= [Ψ, inr x :: s]close cl_tm cl_en). 
+    * subst. apply Upd.  
+    * assumption.  
 (* Lam *)
 - intros. apply t_refl. 
 (* App *)
-- intros. apply t_step with (y:=b2s (⟨Φ ⟩ close M e) (inl (close N e)::s)). 
+- intros. apply t_step with (y:=(st Φ0 (inl (close N e)::s)) (close M e)). 
   + apply App. 
   + apply refl_trans_clos_app with (y:=b2s (⟨Ψ, f ↦ {close N e, ne} ⟩ close B f) s).
     * apply t_step2 with (y:=b2s (⟨Ψ ⟩ close (db.lam B) ne) (inl (close N e):: s)).
       -- simpl. rename e into E. rename s into S. 
          apply Abs with (b:=B) (e:=ne) (c:=close N E) (s:= S). 
          assumption. 
-      -- auto. 
-    * auto. 
+      -- apply IHX1. reflexivity. reflexivity.  
+    * simpl. apply IHX2. reflexivity. reflexivity.  
 Qed. 
 
 (*
