cesm_im.v
@@ -1,4 +1,4 @@
-Require Import Unicode.Utf8 util cesm im db db_assembly assembly relations List cem.
+Require Import util cesm im db db_assembly assembly relations List cem.
 Import ListNotations.
 
 Variable new : ∀ (n:nat) (h : im.Heap), sigT (λ w:nat, ∀ i, lt i n → (plus w i) ∉ domain h).
@@ -49,9 +49,9 @@ Lemma cesm_im : ∀ v s s',
   state_rel s s' → 
   cesm.step s v → 
   sigT (λ v', refl_trans_clos im.step s' v' * state_rel v v').
-intros v s s' r h. generalize dependent r. generalize dependent s'.  induction
-h; intros. 
-- inversion r. subst. inversion X0. subst. destruct s'. simpl in *. subst.   
+intros v s s' r h. induce h. 
+- invert r. invert X. 
+  
 Admitted.
 
 Lemma cesm_im_assemble : ∀ t v v', 
